backend/ValueAnalysis.v
@@ -956,7 +956,7 @@ Proof.
   intros until am; intros EC GENV ARGS RO MM NOSTACK.
   (* Part 1: using ec_mem_inject *)
   exploit (@external_call_mem_inject ef _ _ ge vargs m t vres m' (inj_of_bc bc) m vargs).
-  apply inj_of_bc_preserves_globals; auto.
+  apply inj_of_bc_inject_globals; auto.
   exact EC.
   eapply mmatch_inj; eauto. eapply mmatch_below; eauto.
   revert ARGS. generalize vargs.
